src/typed_ast.ml
@@ -358,7 +358,7 @@ and def_aux =
   | OpenImportTarget of Ast.open_import * targets_opt * (lskips * string) list
   | Indreln of lskips * targets_opt * indreln_name lskips_seplist * indreln_rule lskips_seplist
   | Val_spec of val_spec
-  | Class of lskips * lskips * name_l * tnvar * Path.t * lskips * class_val_spec list * lskips
+  | Class of Ast.class_decl * lskips * name_l * tnvar * Path.t * lskips * class_val_spec list * lskips
   (* The v_env, name and Path/tyvar list are for converting the instance into a module. *)
   | Instance of Ast.instance_decl * Types.instance_ref * instschm * val_def list * lskips 
   | Comment of def
@@ -655,9 +655,12 @@ let rec def_alter_init_lskips (lskips_f : lskips -> lskips * lskips) (((d,s),l,l
       | Val_spec(sk1,n,n_ref,ao,sk2,ts) ->
           let (s_new, s_ret) = lskips_f sk1 in
             res (Val_spec(s_new,n,n_ref,ao,sk2,ts)) s_ret
-      | Class(sk1,sk2,n,tvar,class_ty,sk3,body,sk4) ->
+      | Class(Ast.Class_decl sk1,sk2,n,tvar,class_ty,sk3,body,sk4) ->
           let (s_new, s_ret) = lskips_f sk1 in
-            res (Class(s_new,sk2,n,tvar,class_ty,sk3,body,sk4)) s_ret
+            res (Class(Ast.Class_decl s_new,sk2,n,tvar,class_ty,sk3,body,sk4)) s_ret
+      | Class(Ast.Class_inline_decl (sk1, sk1'),sk2,n,tvar,class_ty,sk3,body,sk4) ->
+          let (s_new, s_ret) = lskips_f sk1 in
+            res (Class(Ast.Class_inline_decl (s_new,sk1'),sk2,n,tvar,class_ty,sk3,body,sk4)) s_ret
       | Instance(Ast.Inst_decl sk1,i_ref,is,ds,sk2) ->
           let (s_new, s_ret) = lskips_f sk1 in
             res (Instance(Ast.Inst_decl s_new,i_ref,is,ds,sk2)) s_ret
